commit

Src/prover/Set.lean
@@ -17,10 +17,18 @@ def not_mem (a b : Set) : Prop :=
 infix:50 (priority := high) " ∉ " => not_mem
 
 def empty (a : Set) : Prop :=
-¬∃ (b : Set), b ∈ a
+¬∃ b, b ∈ a
 
 def nonempty (a : Set) : Prop :=
 ¬empty a
+
+def is_set_succ (n n1 : Set) : Prop :=
+∀ a, a ∈ n1 ↔ a ∈ n ∨ a = n1
+
+def subset (a b : Set) : Prop :=
+∀ c, c ∈ a → c ∈ b
+
+infix:50 (priority := high) " ⊆ " => subset
 
 -- Axioms
 
@@ -28,9 +36,26 @@ axiom ax_ext {a b} : (∀ c, c ∈ a ↔ c ∈ b) → a = b
 axiom ax_reg {a} : nonempty a → ∃ b, b ∈ a ∧ ¬∃ c, c ∈ b ∧ c ∈ a
 axiom ax_spec (P : Set → Prop) a : ∃ b, ∀ c, c ∈ b ↔ c ∈ a ∧ P c
 axiom ax_union a : ∃ b, ∀ c d, (d ∈ c ∧ c ∈ a) → d ∈ b
--- axiom ax_rep (P : Set → Set → Prop) {a} :
+axiom ax_rep (P : Set → Set → Prop) {a} : (∀ b, b ∈ a → ∃! c, P b c) →
+  ∃ b, ∀ c, c ∈ a → ∃ d, d ∈ b ∧ P c d
+axiom ax_inf : ∃ a b, empty b ∧ b ∈ a ∧ ∀ c, c ∈ a → ∀ d, is_set_succ c d → d ∈ a
+axiom ax_pow : ∀ a, ∃ b, ∀ c, c ⊆ a → c ∈ b
+
+-- Choice
+
+axiom some {α : Type} {P : α → Prop} : (∃ (x : α), P x) → α
+axiom some_spec {α : Type} {P : α → Prop} (h : ∃ (x : α), P x) : P (some h)
 
 -- Theorems
+
+theorem not_empty a : ¬empty a ↔ nonempty a :=
+iff_refl
+
+theorem not_nonempty a : ¬nonempty a ↔ empty a :=
+iff_intro not_not_elim not_not_intro
+
+theorem subset_refl a : a ⊆ a :=
+λ _ => id
 
 -----
 
